## length [1,2,3]
### 定義
```haskell
length :: [a] -> Int
length [] = 0
length (_:xs) = 1 + length xs
```

### 簡約
```haskell
length [1,2,3]
= 1 + length [2,3]
= 1 + 1 + length [3]
= 1 + 1 + 1 + length []
= 1 + 1 + 1 + 0
= 3
```

## drop 3 [1,2,3,4,5]
### 定義
```haskell
drop :: Int -> [a] -> [a]
drop 0 xs = xs
drop (n + 1) []
drop (n + 1) (_:xs) = drop n xs
```

### 簡約
```haskell
drop 3 [1,2,3,4,5]
= drop 2 [2,3,4,5]
= drop 1 [3,4,5]
= drop 0 [4,5]
= [4,5]
```

## init [1,2,3]
### 定義
```haskell
init :: [a] -> [a]
init [_] = []
init (x:xs) = x : init xs
```

### 簡約
```haskell
init [1,2,3]
= 1 : init [2,3]
= 1 : 2 : init [3]
= 1 : 2 : []
= [1,2]
```
